Test/tutorial/ImpVerifiedCompiler/SimulationRelationCont.dfy
@@ -103,4 +103,3 @@ lemma compile_cont_Kwhile_inv(C: code, b: bexp, c: com, k: cont, pc: nat, s: sto
 	}
 	
 }
-
